theories/νSet/νGpd.v
@@ -1,0 +1,650 @@
+(** Groupoid-level variant of the νSet construction. *)
+
+From Stdlib Require Import Logic.FunctionalExtensionality.
+
+Set Warnings "-notation-overridden".
+From Bonak Require Import SigT RewLemmas HSet HGpd Notation LeSProp νSet.νSet.
+Import Bonak.νSet.νSet.
+
+Set Primitive Projections.
+Set Printing Projections.
+Set Keyed Unification.
+
+Module νGpd (A : AritySig).
+Import A.
+
+Notation "{ x & P }" := (gsigT (fun x => P%type)): type_scope.
+Notation "{ x : A & P }" := (gsigT (A := A) (fun x => P%type)): type_scope.
+
+(** The type of lists {frame(n,0);...;frame(n,p-1)} for arbitrary k := n-p
+    (the non-mandatory dependency in k is useful for type inference) *)
+
+Fixpoint mkFrameTypes p k: Type :=
+  match p with
+  | 0 => unit
+  | S p => { frames: mkFrameTypes p k.+1 &T HGpd }
+  end.
+
+(** The type of lists {painting(n,0);...;painting(n,p-1)} for n := k+p *)
+
+Fixpoint mkPaintingTypes p k: mkFrameTypes p k -> Type :=
+  match p with
+  | 0 => fun _ => unit
+  | S p => fun frames =>
+    { paintings: mkPaintingTypes p k.+1 frames.1 &T frames.2 -> HGpd }
+  end.
+
+(** A helper type so as to mutually build the types of restrFrames and
+    the body of frames using a single fixpoint *)
+
+Class RestrFrameTypeBlock p k := {
+  RestrFrameTypesDef: Type;
+  FrameDef: RestrFrameTypesDef -> mkFrameTypes p.+1 k;
+}.
+
+(**
+For n and p<=n be given, and assuming {frame(n,0);...;frame(n,p)} and
+{painting(n,0);...;painting(n,p)}, we build the list of pairs:
+- of the types RestrFrameTypes(n,p) of the list
+  {restrFrame(n,0);...;restrFrame(n,p-1)}
+  (represented as an inhabitant of a sigma-type
+   {R:RestrFrameTypes(n,0) & ... & RestrFrameTypes(n,p-1)})
+- and of the list {frame(n+1,0);...;frame(n+1,p)} in function of effective
+  restrFrames of type RestrFrameTypes(n,p)
+
+That is, we build:
+- p = 0 : { RestrFrameTypes(n,0..0-1) := unit ;
+                  (which denotes the empty list of restrFrameTypes)
+            Frames(n+1,0..0)(restrFrames^n_{0..0-1}) := {unit}
+                  (representing lists by Sigma-types) }
+- p = 1 : { RestrFrameTypes(n,0..0) = {_:unit & restrFrameType(n,0)} ;
+                  (thus denoting the singleton list {restrFrameType(n,0})
+            Frames(n+1,0..1)(restrFrames(n,0..0) :=
+                  {unit;{d:Frame(n,0)&Painting(n,0)(restrFrame(n,0)(d)}} }
+- ...
+- p     : { RestrFrameTypes(n,0..p-1) =
+              {RestrFrameType(n,0) & ... & RestrFrameType(n,p-1)} ;
+            Frames(n+1,0..p)(restrFrames(n,0..p-1)) :=
+              {frame(n+1,0);...;frame(n+1,p)} }
+
+  In practise, it is convenient to work with the difference k := n-p
+  rather than n itself. So, below, k is the difference.
+*)
+
+Generalizable Variables p k frames.
+
+Definition mkRestrFrameTypesStep `(frames: mkFrameTypes p.+1 k)
+  (prev: RestrFrameTypeBlock p k.+1) :=
+  { R: prev.(RestrFrameTypesDef) &T
+    forall q (Hq: q <= k) (ε: arity), (prev.(FrameDef) R).2 -> frames.2 }.
+
+Definition mkLayer `{paintings: mkPaintingTypes p.+1 k frames}
+  {prev: RestrFrameTypeBlock p k.+1}
+  (restrFrames: mkRestrFrameTypesStep frames prev)
+  (d: (prev.(FrameDef) restrFrames.1).2) :=
+  gforall ε, paintings.2 (restrFrames.2 0 leR_O ε d).
+
+Fixpoint mkRestrFrameTypesAndFrames {p k}:
+  forall `(paintings: mkPaintingTypes p k frames), RestrFrameTypeBlock p k :=
+  match p with
+  | 0 => fun frames paintings =>
+    {|
+      RestrFrameTypesDef := unit;
+      FrameDef _ := (tt; gunit): mkFrameTypes 1 k
+    |}
+  | p.+1 => fun frames paintings =>
+    let prev :=
+      mkRestrFrameTypesAndFrames paintings.1 in
+    let frames' := prev.(FrameDef) in
+    {|
+      RestrFrameTypesDef := mkRestrFrameTypesStep frames prev;
+      FrameDef R :=
+        (frames' R.1; { d: (frames' R.1).2 &
+          mkLayer (paintings := paintings) R d }): mkFrameTypes p.+2 k
+    |}
+  end.
+
+Definition mkRestrFrameTypes `(paintings: mkPaintingTypes p k frames) :=
+  (mkRestrFrameTypesAndFrames paintings).(RestrFrameTypesDef).
+
+Class DepsRestr p k := {
+  _frames: mkFrameTypes p k;
+  _paintings: mkPaintingTypes p k _frames;
+  _restrFrames: mkRestrFrameTypes _paintings;
+}.
+
+Instance toDepsRestr `{paintings: mkPaintingTypes p k frames}
+  (restrFrames: mkRestrFrameTypes paintings) : DepsRestr p k :=
+  {| _restrFrames := restrFrames |}.
+
+#[local]
+Instance proj1DepsRestr `(deps: DepsRestr p.+1 k): DepsRestr p k.+1 :=
+{|
+  _frames := deps.(_frames).1;
+  _paintings := deps.(_paintings).1;
+  _restrFrames := deps.(_restrFrames).1;
+|}.
+
+Declare Scope depsrestr_scope.
+Delimit Scope depsrestr_scope with depsrestr.
+Bind Scope depsrestr_scope with DepsRestr.
+Notation "x .(1)" := (proj1DepsRestr x%_depsrestr)
+  (at level 1, left associativity, format "x .(1)"): depsrestr_scope.
+
+Definition mkFrames `(deps: DepsRestr p k): mkFrameTypes p.+1 k :=
+  (mkRestrFrameTypesAndFrames
+    deps.(_paintings)).(FrameDef) deps.(_restrFrames).
+
+Definition mkFrame `(deps: DepsRestr p k): HGpd := (mkFrames deps).2.
+
+Inductive DepsRestrExtension p: forall k, DepsRestr p k -> Type :=
+| TopRestrDep {deps} (E: mkFrame deps -> HGpd): DepsRestrExtension p 0 deps
+| AddRestrDep {k} deps:
+  DepsRestrExtension p.+1 k deps -> DepsRestrExtension p k.+1 deps.(1).
+
+Arguments TopRestrDep {p deps}.
+Arguments AddRestrDep {p k} deps.
+
+Declare Scope extra_depsrestr_scope.
+Delimit Scope extra_depsrestr_scope with extradepsrestr.
+Bind Scope extra_depsrestr_scope with DepsRestrExtension.
+Notation "( x ; y )" := (AddRestrDep x y)
+  (at level 0, format "( x ; y )"): extra_depsrestr_scope.
+
+(* Example: if p := 0, extraDeps := ({},E) mkPainting:= {E} *)
+
+Generalizable Variables deps.
+
+Fixpoint mkPainting `(extraDeps: DepsRestrExtension p k deps):
+  mkFrame deps -> HGpd :=
+  match extraDeps with
+  | TopRestrDep E => fun d => E d
+  | AddRestrDep deps extraDeps => fun (d: mkFrame deps.(1)) =>
+      {l: mkLayer deps.(_restrFrames) d & mkPainting extraDeps (d; l)}
+  end.
+
+Fixpoint mkPaintingsPrefix {p k}:
+  forall `(extraDeps: DepsRestrExtension p k deps),
+    mkPaintingTypes p k.+1 (mkFrames deps).1 :=
+  match p with
+  | 0 => fun _ _ => tt
+  | S p => fun deps extraDeps =>
+      (mkPaintingsPrefix (deps; extraDeps)%extradepsrestr;
+       mkPainting (deps; extraDeps)%extradepsrestr)
+  end.
+
+Definition mkPaintings {p k}: forall `(extraDeps: DepsRestrExtension p k deps),
+  mkPaintingTypes p.+1 k (mkFrames deps) :=
+  fun deps extraDeps => (mkPaintingsPrefix extraDeps; mkPainting extraDeps).
+
+Definition mkRestrPaintingType
+  `(extraDeps: DepsRestrExtension p.+1 k deps) :=
+  forall q (Hq: q <= k) ε (d: mkFrame deps.(1)),
+  (mkPaintings (deps; extraDeps)).2 d ->
+  deps.(_paintings).2 (deps.(_restrFrames).2 q Hq ε d).
+
+Fixpoint mkRestrPaintingTypes {p}:
+  forall `(extraDeps: DepsRestrExtension p k deps), Type :=
+  match p with
+  | 0 => fun _ _ _ => unit
+  | S p =>
+    fun k deps extraDeps =>
+    { _: mkRestrPaintingTypes (deps; extraDeps) &T
+      mkRestrPaintingType extraDeps }
+  end.
+
+(** A helper type so as to mutually build the types of cohFrames and
+    the body of restrFrames using a single fixpoint *)
+
+Class CohFrameTypeBlock `{extraDeps: DepsRestrExtension p k deps} := {
+  CohFrameTypesDef: Type;
+  RestrFramesDef: CohFrameTypesDef -> mkRestrFrameTypes (mkPaintings extraDeps)
+}.
+
+(** Auxiliary definitions to mutually build cohFrameTypes and restrFrames *)
+
+Definition mkCohFrameTypesStep `{extraDeps: DepsRestrExtension p.+1 k deps}
+  (prev: CohFrameTypeBlock (extraDeps := (deps; extraDeps))): Type :=
+  { Q: prev.(CohFrameTypesDef) &T
+    forall q (Hq: q <= k) r (Hr: r <= q) (ε ω: arity) d,
+    deps.(_restrFrames).2 q Hq ε
+      ((prev.(RestrFramesDef) Q).2 r (Hr ↕ (↑ Hq)) ω d) =
+    deps.(_restrFrames).2 r (Hr ↕ Hq) ω
+      ((prev.(RestrFramesDef) Q).2 q.+1 (⇑ Hq) ε d) }.
+
+Definition mkRestrLayer `{extraDeps: DepsRestrExtension p.+1 k deps}
+  (restrPaintings: mkRestrPaintingTypes extraDeps)
+  {prev: CohFrameTypeBlock (extraDeps := (deps; extraDeps))}
+  (cohFrames: mkCohFrameTypesStep prev)
+  q (Hq: q <= k) (ε: arity)
+  (d: mkFrame (toDepsRestr (prev.(RestrFramesDef) cohFrames.1)).(1)):
+  mkLayer (prev.(RestrFramesDef) cohFrames.1) d -> mkLayer deps.(_restrFrames)
+    ((prev.(RestrFramesDef) cohFrames.1).2 q.+1 (⇑ Hq) ε d) :=
+  fun l ω => rew [deps.(_paintings).2] cohFrames.2 q Hq 0 leR_O ε ω d in
+             restrPaintings.2 q Hq ε _ (l ω).
+
+(** Under previous assumptions, and, additionally:
+    - {restrPainting(n,0);...;restrPainting(n,p-1)}
+    we mutually build the pair of:
+    - the list of types for {cohFrame(n,0);...;cohFrame(n,p-1)}
+    - definitions of {restrFrame(n+1,0);...;restrFrame(n+1,p)} *)
+
+Fixpoint mkCohFrameTypesAndRestrFrames {p k}:
+  forall `{extraDeps: DepsRestrExtension p k deps}
+  (restrPaintings: mkRestrPaintingTypes extraDeps), CohFrameTypeBlock :=
+  match p with
+  | 0 =>
+    fun deps extraDeps restrPaintings =>
+    {|
+      CohFrameTypesDef := unit;
+      RestrFramesDef _ := (tt; fun _ _ _ _ => tt)
+    |}
+  | S p =>
+    fun deps extraDeps restrPaintings =>
+    let prev := mkCohFrameTypesAndRestrFrames restrPaintings.1 in
+    let restrFrames := prev.(RestrFramesDef) in
+    {|
+      CohFrameTypesDef := mkCohFrameTypesStep prev;
+      RestrFramesDef Q :=
+      let restrFrame q (Hq: q <= k) ε
+        (d: mkFrame (toDepsRestr (restrFrames Q.1))) :=
+          ((restrFrames Q.1).2 q.+1 (⇑ Hq) ε d.1;
+           mkRestrLayer restrPaintings Q q _ ε d.1 d.2)
+      in (restrFrames Q.1; restrFrame)
+    |}
+  end.
+
+(* Example: if p := 0, extraDeps := ({},E)
+   mkCohFrameTypes := {} *)
+
+Definition mkCohFrameTypes `{extraDeps: DepsRestrExtension p k deps}
+  (restrPaintings: mkRestrPaintingTypes extraDeps) :=
+  (mkCohFrameTypesAndRestrFrames restrPaintings).(CohFrameTypesDef).
+
+Class DepsCohs p k := {
+  _deps: DepsRestr p k;
+  _extraDeps: DepsRestrExtension p k _deps;
+  _restrPaintings: mkRestrPaintingTypes _extraDeps;
+  _cohs: mkCohFrameTypes _restrPaintings;
+}.
+
+#[local]
+Instance toDepsCohs `{extraDeps: DepsRestrExtension p k deps}
+  {restrPaintings: mkRestrPaintingTypes extraDeps}
+  (cohs: mkCohFrameTypes restrPaintings): DepsCohs p k :=
+  {| _cohs := cohs |}.
+
+#[local]
+Instance proj1DepsCohs `(depsCohs: DepsCohs p.+1 k): DepsCohs p k.+1 :=
+{|
+  _deps := depsCohs.(_deps).(1);
+  _extraDeps := (depsCohs.(_deps); depsCohs.(_extraDeps));
+  _restrPaintings := depsCohs.(_restrPaintings).1;
+  _cohs := depsCohs.(_cohs).1;
+|}.
+
+Declare Scope depscohs_scope.
+Delimit Scope depscohs_scope with depscohs.
+Bind Scope depscohs_scope with DepsCohs.
+Notation "x .(1)" := (proj1DepsCohs x%depscohs)
+  (at level 1, left associativity, format "x .(1)"): depscohs_scope.
+
+(** The restrFrame(n+1,0..p) component of the fixpoint *)
+
+Definition mkRestrFrames `{depsCohs: DepsCohs p k} :=
+  (mkCohFrameTypesAndRestrFrames depsCohs.(_restrPaintings)).(RestrFramesDef)
+    depsCohs.(_cohs).
+
+(** For n=p+k, we combine mkFrames (that is frames(n+1,p)),
+    mkPaintings (that is paintings(n+1,p)) and restrFrames
+    (that is restrFrames(n+1,p)) to build "dependencies" at the next
+    level, that is a deps(n+1,p).
+    That is, from:
+     - {frame(n,0);...;frame(n,p-1)}
+     - {painting(n,0);...;painting(n,p-1)}
+     - {restrFrame(n,0);...;restrFrame(n,p-1)} for p<=n+1
+     (forming a "deps"), and
+     - {frame(n,p);...;frame(n,n)}
+     - {painting(n,p);...;painting(n,n)}
+     - {restrFrame(n,p);...;restrFrame(n,n)}
+     - E:frame(n+1,n+1) -> HGpd
+     (forming an "extraDeps")
+     we form:
+     - {frame(n+1,0);...;frame(n+1,p)} (built by mkFrames)
+     - {painting(n+1,0);...;painting(p+n,p)} (built by mkPaintings)
+     - {restrFrame(n+1,0);...;restrFrame(n+1,p)} (built by mkRestrFrames)
+
+   Example: if p := 0, extraDeps := ({},E), restrPaintings := {}, cohs := {}
+   then mkDepsRestr := {frames'':={unit};
+                        paintings'':={E};
+                        restrFrames':={λqω().()}}
+   (where restrFrames' is presented as a dependent pair, i.e. ((),λqω().()) *)
+
+Definition mkDepsRestr `{depsCohs: DepsCohs p k} :=
+  toDepsRestr mkRestrFrames.
+
+(** Deducing restrFrame(n+1,p) *)
+
+(** Note that we use mkRestrFrames(n+1,p) both to build frame(n+2,p) and
+    restrFrame(n+1,p) : frame(n+2,p) -> frame(n+1,p), according to the
+    circularity between Frames and RestrFrameTypes.
+    But now, thanks to restrPaintings and cohFrames, we have an effective
+    definition of RestrFrame(n+1,p) and the circular dependency of
+    frame(n+2,p) with an inhabitant RestrFrame(n+1,p) of RestrFrameType(n+1,p)
+    is gone.
+ *)
+
+Definition mkRestrFrame `{depsCohs: DepsCohs p k}:
+  forall q (Hq: q <= k) (ε: arity),
+  mkFrame mkDepsRestr.(1) -> mkFrame depsCohs.(_deps) :=
+  mkRestrFrames.2.
+
+Inductive DepsCohsExtension p: forall k (depsCohs: DepsCohs p k), Type :=
+| TopCohDep `{depsCohs: DepsCohs p 0}
+  (E: mkFrame mkDepsRestr -> HGpd):
+  DepsCohsExtension p 0 depsCohs
+| AddCohDep {k} (depsCohs: DepsCohs p.+1 k):
+  DepsCohsExtension p.+1 k depsCohs -> DepsCohsExtension p k.+1 depsCohs.(1).
+
+Arguments TopCohDep {p depsCohs}.
+Arguments AddCohDep {p k}.
+
+Declare Scope extra_depscohs_scope.
+Delimit Scope extra_depscohs_scope with extradepscohs.
+Bind Scope extra_depscohs_scope with DepsCohsExtension.
+Notation "( x ; y )" := (AddCohDep x y)
+  (at level 0, format "( x ; y )"): extra_depscohs_scope.
+
+Generalizable Variables depsCohs.
+
+Fixpoint mkExtraDeps `(extraDepsCohs: DepsCohsExtension p k depsCohs):
+  DepsRestrExtension p.+1 k mkDepsRestr.
+Proof.
+  destruct extraDepsCohs.
+  - now constructor.
+  - apply (AddRestrDep mkDepsRestr
+    (mkExtraDeps p.+1 k depsCohs extraDepsCohs)).
+Defined.
+
+Fixpoint mkRestrPainting `(extraDepsCohs: DepsCohsExtension p k depsCohs)
+  q {struct q}:
+  forall (Hq: q <= k) ε (d: mkFrame mkDepsRestr.(1)),
+    (mkPaintings (mkDepsRestr; mkExtraDeps extraDepsCohs)).2 d ->
+    mkDepsRestr.(_paintings).2 (mkDepsRestr.(_restrFrames).2 q Hq ε d) :=
+  match q with
+  | 0 => fun _ ε _ '(l; _) => l ε
+  | q.+1 =>
+    match extraDepsCohs with
+    | TopCohDep E => fun Hq _ _ _ => match leR_O_contra Hq with end
+    | AddCohDep depsCohs extraDepsCohs => fun Hq ε d '(l; c) =>
+      (mkRestrLayer depsCohs.(_restrPaintings) depsCohs.(_cohs) q (⇓ Hq) ε d l;
+       mkRestrPainting extraDepsCohs q (⇓ Hq) ε (d; l) c)
+    end
+  end.
+
+Fixpoint mkRestrPaintingsPrefix {p k}:
+  forall `(extraDepsCohs: DepsCohsExtension p k depsCohs),
+  mkRestrPaintingTypes
+    (mkDepsRestr; mkExtraDeps extraDepsCohs)%extradepsrestr :=
+  match p with
+  | 0 => fun _ _ => tt
+  | S p =>
+    fun depsCohs extraDepsCohs =>
+      (mkRestrPaintingsPrefix (depsCohs; extraDepsCohs)%extradepscohs;
+       mkRestrPainting (depsCohs; extraDepsCohs)%extradepscohs)
+  end.
+
+Definition mkRestrPaintings {p k}:
+  forall `(extraDepsCohs: DepsCohsExtension p k depsCohs),
+  mkRestrPaintingTypes (mkExtraDeps extraDepsCohs) :=
+  fun depsCohs extraDepsCohs => (mkRestrPaintingsPrefix extraDepsCohs; mkRestrPainting extraDepsCohs).
+
+(** The groupoid-level replacement for the old [mkCoh2Frame] UIP proof:
+    this is now explicit 2-dimensional frame coherence data. *)
+
+Definition mkCoh2FrameType
+  `(extraDepsCohs: DepsCohsExtension p.+1 k depsCohs)
+  (prevCohFrames: mkCohFrameTypes
+     (extraDeps := (mkDepsRestr; mkExtraDeps extraDepsCohs))
+     (mkRestrPaintings extraDepsCohs).1): Type :=
+  forall q (Hq: q <= k) r (Hr: r <= q) s (Hs: s <= r) (ε ω 𝛉: arity)
+    (d: mkFrame (mkDepsRestr (depsCohs := toDepsCohs prevCohFrames.1)).(1)),
+  f_equal
+    (fun x => depsCohs.(_deps).(_restrFrames).2 q _ ε x)
+    (prevCohFrames.2 r (Hr ↕ ↑ Hq) s Hs ω 𝛉 d)
+  • (depsCohs.(_cohs).2 q Hq s (Hs ↕ Hr) ε 𝛉
+      (mkRestrFrame r.+1 (⇑ (Hr ↕ ↑ Hq)) ω d)
+  • f_equal
+      (fun x => depsCohs.(_deps).(_restrFrames).2 s (Hs ↕ (Hr ↕ Hq)) 𝛉 x)
+      (prevCohFrames.2 q.+1 (⇑ Hq) r.+1 (⇑ Hr) ε ω d)) =
+  depsCohs.(_cohs).2 q Hq r Hr ε ω
+    (mkRestrFrame s (↑ (↑ (Hs ↕ (Hr ↕ Hq)))) 𝛉 d)
+  • (f_equal
+      (fun x => depsCohs.(_deps).(_restrFrames).2 r _ ω x)
+      (prevCohFrames.2 q.+1 (⇑ Hq) s (↑ (Hs ↕ Hr)) ε 𝛉 d)
+  • depsCohs.(_cohs).2 r (Hr ↕ Hq) s Hs ω 𝛉
+      (mkRestrFrame q.+2 (⇑ (⇑ Hq)) ε d)).
+
+Definition mkCohPaintingType
+  `(extraDepsCohs: DepsCohsExtension p.+1 k depsCohs) :=
+  forall q (Hq: q <= k) r (Hr: r <= q) (ε ω: arity)
+    (d: mkFrame mkDepsRestr.(1))
+    (c: (mkPaintings (mkDepsRestr;
+      mkExtraDeps (depsCohs; extraDepsCohs))).2 d),
+  rew [depsCohs.(_deps).(_paintings).2] depsCohs.(_cohs).2 q Hq r Hr ε ω d in
+  depsCohs.(_restrPaintings).2 q Hq ε _
+    ((mkRestrPaintings (depsCohs; extraDepsCohs)).2 r _ ω d c) =
+  depsCohs.(_restrPaintings).2 r (Hr ↕ Hq) ω _
+    ((mkRestrPaintings (depsCohs; extraDepsCohs)).2 q.+1 _ ε d c).
+
+Fixpoint mkCohPaintingTypes {p}:
+  forall `(extraDepsCohs: DepsCohsExtension p k depsCohs), Type :=
+  match p with
+  | 0 => fun _ _ _ => unit
+  | S p =>
+    fun k depsCohs extraDepsCohs =>
+    { R: mkCohPaintingTypes (depsCohs; extraDepsCohs) &T
+         mkCohPaintingType extraDepsCohs }
+  end.
+
+Definition mkCohLayer `{extraDepsCohs: DepsCohsExtension p.+1 k depsCohs}
+  (cohPaintings: mkCohPaintingTypes extraDepsCohs)
+  {prevCohFrames: mkCohFrameTypes
+    (extraDeps := (mkDepsRestr; mkExtraDeps extraDepsCohs))
+    (mkRestrPaintings extraDepsCohs).1}
+  (coh2Frame: mkCoh2FrameType extraDepsCohs prevCohFrames)
+  q {Hq: q <= k} r {Hr: r <= q} (ε ω: arity)
+  (d: mkFrame (mkDepsRestr (depsCohs := toDepsCohs prevCohFrames.1)).(1))
+  (l: mkLayer mkRestrFrames d):
+  rew [mkLayer _] prevCohFrames.2 q.+1 (⇑ Hq) r.+1 (⇑ Hr) ε ω d in
+    mkRestrLayer depsCohs.(_restrPaintings) depsCohs.(_cohs) q Hq ε _
+      (mkRestrLayer (mkRestrPaintings extraDepsCohs).1 _ r (Hr ↕ ↑ Hq) ω d l) =
+    mkRestrLayer depsCohs.(_restrPaintings) depsCohs.(_cohs) r (Hr ↕ Hq) ω _
+      (mkRestrLayer (mkRestrPaintings extraDepsCohs).1 _ q.+1 (⇑ Hq) ε d l).
+Proof.
+  apply functional_extensionality_dep; intros 𝛉.
+  rewrite <- map_subst_app. unfold mkRestrLayer; simpl.
+  rewrite
+    <- map_subst with (f := fun x => depsCohs.(_restrPaintings).2 q Hq ε x),
+    <- map_subst with
+        (f := fun x => depsCohs.(_restrPaintings).2 r (Hr ↕ Hq) ω x),
+    -> rew_map with (P := fun x => depsCohs.(_deps).(_paintings).2 x)
+        (f := fun x => depsCohs.(_deps).(_restrFrames).2 O leR_O 𝛉 x),
+    -> rew_map with (P := fun x => depsCohs.(_deps).(_paintings).2 x)
+        (f := fun x => depsCohs.(_deps).(_restrFrames).2 r
+          (Hr ↕ Hq) ω x),
+    -> rew_map with (P := fun x => depsCohs.(_deps).(_paintings).2 x)
+        (f := fun x => depsCohs.(_deps).(_restrFrames).2 q _ ε x),
+    <- cohPaintings.2.
+  repeat rewrite rew_compose.
+  apply rew_swap with (P := fun x => depsCohs.(_deps).(_paintings).2 x).
+  rewrite rew_app_rl. now trivial.
+  now apply (coh2Frame q Hq r Hr 0 leR_O ε ω 𝛉 d).
+Defined.
+
+Class Coh2FrameTypeBlock `{extraDepsCohs: DepsCohsExtension p k depsCohs}
+  (cohPaintings: mkCohPaintingTypes extraDepsCohs) := {
+  Coh2FrameTypesDef: Type;
+  CohFramesDef: Coh2FrameTypesDef -> mkCohFrameTypes (mkRestrPaintings extraDepsCohs);
+}.
+
+Definition mkCoh2FrameTypesStep
+  `{extraDepsCohs: DepsCohsExtension p.+1 k depsCohs}
+  (cohPaintings: mkCohPaintingTypes extraDepsCohs)
+  (prev: Coh2FrameTypeBlock
+    (extraDepsCohs := (depsCohs; extraDepsCohs)%extradepscohs)
+    cohPaintings.1): Type :=
+  { R: prev.(Coh2FrameTypesDef) &T
+    mkCoh2FrameType extraDepsCohs (prev.(CohFramesDef) R) }.
+
+Fixpoint mkCoh2FrameTypesAndCohFrames {p k}:
+  forall `{extraDepsCohs: DepsCohsExtension p k depsCohs}
+  (cohPaintings: mkCohPaintingTypes extraDepsCohs), Coh2FrameTypeBlock cohPaintings.
+Proof.
+  destruct p.
+  - intros depsCohs extraDepsCohs cohPaintings.
+    unshelve econstructor.
+    + now exact unit.
+    + intros _. unshelve esplit. now exact tt. now intros.
+  - intros depsCohs extraDepsCohs cohPaintings.
+    set (prev := mkCoh2FrameTypesAndCohFrames p k.+1
+      depsCohs.(1)%depscohs
+      (depsCohs; extraDepsCohs)%extradepscohs cohPaintings.1).
+    unshelve econstructor.
+    + now exact (mkCoh2FrameTypesStep cohPaintings prev).
+    + intros Q.
+      set (h := prev.(CohFramesDef) Q.1).
+      unshelve esplit. now exact h.
+      intros q Hq r Hr ε ω d.
+      unshelve eapply eq_existT_curried.
+      * now exact (h.2 q.+1 (⇑ Hq) r.+1 (⇑ Hr) ε ω d.1).
+      * now exact (mkCohLayer cohPaintings Q.2 q r ε ω d.1 d.2).
+Defined.
+
+Definition mkCoh2FrameTypes `{extraDepsCohs: DepsCohsExtension p k depsCohs}
+  (cohPaintings: mkCohPaintingTypes extraDepsCohs) :=
+  (mkCoh2FrameTypesAndCohFrames cohPaintings).(Coh2FrameTypesDef).
+
+Definition mkCohFrames `{extraDepsCohs: DepsCohsExtension p k depsCohs}
+  (cohPaintings: mkCohPaintingTypes extraDepsCohs)
+  (coh2Frames: mkCoh2FrameTypes cohPaintings):
+  mkCohFrameTypes (mkRestrPaintings extraDepsCohs) :=
+  (mkCoh2FrameTypesAndCohFrames cohPaintings).(CohFramesDef) coh2Frames.
+
+Class DepsCohs2 p k := {
+  _depsCohs: DepsCohs p k;
+  _extraDepsCohs: DepsCohsExtension p k _depsCohs;
+  _cohPaintings: mkCohPaintingTypes _extraDepsCohs;
+  _coh2Frames: mkCoh2FrameTypes _cohPaintings;
+}.
+
+#[local]
+Instance toDepsCohs2 `{extraDepsCohs: DepsCohsExtension p k depsCohs}
+  {cohPaintings: mkCohPaintingTypes extraDepsCohs}
+  (coh2Frames: mkCoh2FrameTypes cohPaintings): DepsCohs2 p k :=
+  {| _coh2Frames := coh2Frames |}.
+
+#[local]
+Instance proj1DepsCohs2 `(depsCohs2: DepsCohs2 p.+1 k): DepsCohs2 p k.+1 :=
+{|
+  _depsCohs := depsCohs2.(_depsCohs).(1);
+  _extraDepsCohs := (depsCohs2.(_depsCohs); depsCohs2.(_extraDepsCohs));
+  _cohPaintings := depsCohs2.(_cohPaintings).1;
+  _coh2Frames := depsCohs2.(_coh2Frames).1;
+|}.
+
+Declare Scope depscohs2_scope.
+Delimit Scope depscohs2_scope with depscohs2.
+Bind Scope depscohs2_scope with DepsCohs2.
+Notation "x .(1)" := (proj1DepsCohs2 x%depscohs2)
+  (at level 1, left associativity, format "x .(1)"): depscohs2_scope.
+
+#[local]
+Instance mkDepsCohs `(depsCohs2: DepsCohs2 p k): DepsCohs p.+1 k :=
+{|
+  _deps := mkDepsRestr;
+  _extraDeps := mkExtraDeps depsCohs2.(_extraDepsCohs);
+  _restrPaintings := mkRestrPaintings depsCohs2.(_extraDepsCohs);
+  _cohs := mkCohFrames depsCohs2.(_cohPaintings) depsCohs2.(_coh2Frames);
+|}.
+
+Inductive DepsCohs2Extension p: forall k (depsCohs2: DepsCohs2 p k), Type :=
+| TopCoh2Dep `{depsCohs2: DepsCohs2 p 0}
+  (E: mkFrame (mkDepsRestr (depsCohs := mkDepsCohs depsCohs2)) -> HGpd)
+  : DepsCohs2Extension p 0 depsCohs2
+| AddCoh2Dep {k} (depsCohs2: DepsCohs2 p.+1 k):
+  DepsCohs2Extension p.+1 k depsCohs2 ->
+  DepsCohs2Extension p k.+1 depsCohs2.(1).
+
+Arguments TopCoh2Dep {p depsCohs2}.
+Arguments AddCoh2Dep {p k}.
+
+Declare Scope extra_depscohs2_scope.
+Delimit Scope extra_depscohs2_scope with extradepscohs2.
+Bind Scope extra_depscohs2_scope with DepsCohs2Extension.
+Notation "( x ; y )" := (AddCoh2Dep x y)
+  (at level 0, format "( x ; y )"): extra_depscohs2_scope.
+
+Fixpoint mkExtraCohs `{depsCohs2: DepsCohs2 p k}
+  (extraDepsCohs2: DepsCohs2Extension p k depsCohs2):
+  DepsCohsExtension p.+1 k (mkDepsCohs depsCohs2).
+Proof.
+  destruct extraDepsCohs2.
+  - now constructor.
+  - apply (AddCohDep (mkDepsCohs depsCohs2)).
+    now exact (mkExtraCohs p.+1 k depsCohs2 extraDepsCohs2).
+Defined.
+
+Fixpoint mkCohPainting `{depsCohs2: DepsCohs2 p k}
+  (extraDepsCohs2: DepsCohs2Extension p k depsCohs2):
+  mkCohPaintingType (mkExtraCohs extraDepsCohs2).
+Proof.
+  red; intros *. destruct c as (l, c), r.
+  - (* r = 0 *)
+    now trivial.
+  - (* r = r'+1, q is necessarily q'+1 and extraDepsCohs non empty *)
+    destruct q; [now contradict Hq |].
+    destruct extraDepsCohs2; [now contradict Hq |].
+    simpl.
+    unshelve eapply (eq_existT_curried_dep
+      (Q := mkPainting depsCohs2.(_depsCohs).(_extraDeps))).
+    + now exact (mkCohLayer depsCohs2.(_cohPaintings) depsCohs2.(_coh2Frames).2
+        q r (Hr := ⇓ Hr) ε ω d l).
+    + now exact (mkCohPainting p.+1 k depsCohs2 extraDepsCohs2
+        q (⇓ Hq) r (⇓ Hr) ε ω (d; l) c).
+Defined.
+
+Fixpoint mkCohPaintings `{depsCohs2: DepsCohs2 p k}
+  (extraDepsCohs2: DepsCohs2Extension p k depsCohs2) {struct p}:
+  mkCohPaintingTypes (mkExtraCohs extraDepsCohs2).
+Proof.
+  destruct p.
+  - unshelve esplit. now exact tt.
+    now exact (mkCohPainting extraDepsCohs2).
+  - unshelve esplit. now exact (mkCohPaintings p k.+1
+      depsCohs2.(1)%depscohs2 (depsCohs2; extraDepsCohs2)%extradepscohs2).
+    now exact (mkCohPainting extraDepsCohs2).
+Defined.
+
+Fixpoint mkCoh2Frames `{depsCohs2: DepsCohs2 p k}
+  (extraDepsCohs2: DepsCohs2Extension p k depsCohs2):
+  mkCoh2FrameTypes (mkCohPaintings extraDepsCohs2).
+Proof.
+  destruct p.
+  - unshelve esplit.
+    + now exact tt.
+    + intros q Hq r Hr s Hs ε ω θ d.
+      now trivial.
+  - set (h := mkCoh2Frames p k.+1 depsCohs2.(1)%depscohs2
+      (depsCohs2; extraDepsCohs2)%extradepscohs2).
+    unshelve esplit.
+    + now exact h.
+    + intros q Hq r Hr s Hs ε ω θ [d l].
+      rewrite 3 f_equal_eq_existT_curried.
+      rewrite 4 eq_trans_eq_existT_curried.
+      unshelve eapply eq_existT_curried_eq.
+      * now exact (h.2 q.+1 (⇑ Hq) r.+1 (⇑ Hr) s.+1 (⇑ Hs) ε ω θ d).
+      * admit.
+Admitted.
+
+End νGpd.
